\section{Homework 1}

\subsection{Exercise 2.1}
Showing the definition of convexity for arbitrary $k$. $\theta_1 x_1 + \dots + \theta_k x_k \in C$.
\begin{equation}
  \theta_1 x_1 + \dots + \theta_k x_k = \theta_1 x_1 + (1-\theta_1)(\mu_2 x_2 + \mu_3 x_3 + \dots + \mu_k x_k)
\end{equation}
Where each $\mu_n = \frac{\theta_n}{1-\theta_1}$
\\ \\ 
\begin{equation}
  \sum_i \mu_i = \frac{\sum_i \theta_i}{1-\theta_1} = \frac{1-\theta_1}{1-\theta_1} = 1
\end{equation}
\subsection{Exercise 2.2}

\subsection{Exercise 2.5}

\subsection{Exercise 2.7}

\subsection{Exercise 2.8}

\subsection{Exercise 2.11}

\subsection{Exercise 2.12}

\subsection{Exercise 2.15}

